Prove unconditional branch case in the high-level

coq/proof/Simulation.v
@@ -2,6 +2,7 @@ Require Import syntax.
 Require Import alist.
 Require Import FMapWeakList.
 
+Require Import Classical.
 Require Import Coqlib.
 Require Import infrastructure.
 Require Import Metatheory.
@@ -12,10 +13,49 @@ Require Import sflib.
 Require Import paco.
 
 Require Import GenericValues.
-Require Import SimulationLocal.
 
 Set Implicit Arguments.
 
+
+(* TODO: position *)
+Inductive error_state conf st: Prop :=
+| error_state_intro
+    (STUCK: stuck_state conf st)
+    (NFINAL: s_isFinialState conf st = None)
+.
+
+Lemma nerror_stuck_final
+      conf st
+      (NERROR: ~ error_state conf st)
+      (STUCK: stuck_state conf st):
+  exists retval, s_isFinialState conf st = Some retval.
+Proof.
+  destruct (s_isFinialState conf st) eqn:X; eauto.
+  exfalso. apply NERROR. econs; ss.
+Qed.
+
+Lemma nerror_nfinal_nstuck
+      conf st1
+      (NERROR: ~ error_state conf st1)
+      (NFINAL: s_isFinialState conf st1 = None):
+  exists st2 e, sInsn conf st1 st2 e.
+Proof.
+  destruct (classic (stuck_state conf st1)).
+  - contradict NERROR. econs; ss.
+  - apply NNPP in H. ss.
+Qed.
+
+Inductive sInsn_indexed (conf:Config):
+  forall (st1 st2:State) (idx1 idx2:nat) (event:trace), Prop :=
+| sInsn_step
+    st1 st2 idx1 idx2 event
+    (STEP: sInsn conf st1 st2 event):
+    sInsn_indexed conf st1 st2 idx1 idx2 event
+| sInsn_stutter
+    st idx1 idx2
+    (IDX: (idx1 > idx2)%nat):
+    sInsn_indexed conf st st idx1 idx2 E0
+.
 
 Section Sim.
   Variable (conf_src conf_tgt:Config).
@@ -62,7 +102,41 @@ Section Sim.
   Definition sim: _ -> _ -> _ -> Prop :=
     paco3 _sim bot3.
 End Sim.
+Hint Constructors _sim.
 Hint Resolve _sim_mon: paco.
+
+Lemma sop_star_sim
+      conf_src conf_tgt sim idx
+      st1_src st2_src
+      st1_tgt
+      (TAU: sop_star conf_src st1_src st2_src events.E0)
+      (SIM: _sim conf_src conf_tgt sim idx st2_src st1_tgt):
+  _sim conf_src conf_tgt sim idx st1_src st1_tgt.
+Proof.
+  inv SIM.
+  - econs 1; cycle 1; eauto.
+    rewrite <- events.E0_left.
+    eapply opsem_props.OpsemProps.sop_star_trans; eauto.
+  - econs 2; cycle 1; eauto.
+    rewrite <- events.E0_left.
+    eapply opsem_props.OpsemProps.sop_star_trans; eauto.
+  - econs 3; eauto. i. exploit STEP; eauto. i. des.
+    esplits; cycle 1; eauto.
+    rewrite <- events.E0_left.
+    eapply opsem_props.OpsemProps.sop_star_trans; eauto.
+Qed.
+
+Lemma _sim_src_error
+      conf_src conf_tgt sim idx
+      st_src st_tgt
+      (SIM: forall (ERROR_SRC: ~ error_state conf_src st_src),
+          _sim conf_src conf_tgt sim idx
+               st_src st_tgt):
+  _sim conf_src conf_tgt sim idx
+       st_src st_tgt.
+Proof.
+  destruct (classic (error_state conf_src st_src)); eauto.
+Qed.
 
 
 Definition sim_module (module_src module_tgt:module): Prop :=
@@ -72,137 +146,3 @@ Definition sim_module (module_src module_tgt:module): Prop :=
   exists conf_tgt st_tgt idx,
     <<TGT: s_genInitState [module_tgt] main args Mem.empty = Some (conf_tgt, st_tgt)>> /\
     <<SIM: sim conf_src conf_tgt idx st_src st_tgt>>.
-
-Definition return_locals
-           (TD:TargetData)
-           (c:cmd) (retval:option GenericValue) (lc:GVMap): option GVsMap :=
-  match c, retval with
-  | insn_call id0 false _ ct _ _ _, Some retval =>
-    match (fit_gv TD ct) retval with
-    | Some retval' => Some (updateAddAL _ lc id0 retval')
-    | _ => None
-    end
-  | insn_call _ _ _ _ _ _ _, _ => Some lc
-  | _, _ => None
-  end.
-
-Lemma returnUpdateLocals_spec
-      TD c' Result lc lc' gl:
-  returnUpdateLocals TD c' Result lc lc' gl =
-  match getOperandValue TD Result lc gl with
-  | Some retval => return_locals TD c' (Some retval) lc'
-  | None => None
-  end.
-Proof.
-  unfold returnUpdateLocals.
-  destruct (getOperandValue TD Result lc gl); ss.
-Qed.
-
-Inductive sim_local_stack
-          (conf_src conf_tgt:Config):
-  forall (ecs_src ecs_tgt: ECStack) (inv:InvMem.Rel.t), Prop :=
-| sim_local_stack_nil
-    inv:
-    sim_local_stack conf_src conf_tgt nil nil inv
-| sim_local_stack_cons
-    ecs0_src ecs0_tgt inv0
-    inv
-    func_src b_src cmd_src cmds_src term_src locals_src allocas_src ecs_src
-    func_tgt b_tgt cmd_tgt cmds_tgt term_tgt locals_tgt allocas_tgt ecs_tgt
-    (STACK: sim_local_stack conf_src conf_tgt ecs0_src ecs0_tgt inv0)
-    (LE0: InvMem.Rel.le inv0 inv)
-    (CALL_SRC: Instruction.isCallInst cmd_src)
-    (ID: getCmdID cmd_src = getCmdID cmd_tgt)
-    (LOCAL:
-       forall inv' mem'_src mem'_tgt retval'_src retval'_tgt locals'_tgt
-         (LE: InvMem.Rel.le inv inv')
-         (MEM: InvMem.Rel.sem conf_src conf_tgt mem'_src mem'_tgt inv')
-         (RETVAL: TODO.lift2_option (genericvalues_inject.gv_inject inv'.(InvMem.Rel.inject)) retval'_src retval'_tgt)
-         (RETURN_TGT: return_locals conf_tgt.(CurTargetData) cmd_tgt retval'_tgt locals_tgt = Some locals'_tgt),
-       exists idx' locals'_src,
-         <<RETURN_SRC: return_locals conf_src.(CurTargetData) cmd_src retval'_src locals_src = Some locals'_src>> /\
-         <<SIM:
-           sim_local
-             conf_src conf_tgt ecs0_src ecs0_tgt
-             inv' idx'
-             (mkState
-                (mkEC func_src b_src cmds_src term_src locals'_src allocas_src)
-                ecs_src
-                mem'_src)
-             (mkState
-                (mkEC func_tgt b_tgt cmds_tgt term_tgt locals'_tgt allocas_tgt)
-                ecs_tgt
-                mem'_tgt)>>):
-    sim_local_stack
-      conf_src conf_tgt
-      ((mkEC func_src b_src (cmd_src::cmds_src) term_src locals_src allocas_src) :: ecs_src)
-      ((mkEC func_tgt b_tgt (cmd_tgt::cmds_tgt) term_tgt locals_tgt allocas_tgt) :: ecs_tgt)
-      inv
-.
-
-Inductive sim_local_lift
-          (conf_src conf_tgt:Config)
-          (idx:nat) (st_src st_tgt: State): Prop :=
-| sim_local_lift_intro
-    ecs0_src ecs0_tgt inv0
-    inv
-    (STACK: sim_local_stack conf_src conf_tgt ecs0_src ecs0_tgt inv0)
-    (LOCAL: sim_local conf_src conf_tgt ecs0_src ecs0_tgt
-                      inv idx st_src st_tgt)
-    (LE0: InvMem.Rel.le inv0 inv)
-.
-
-Lemma sim_local_lift_sim:
-  sim_local_lift <5= sim.
-Proof.
-  s. intros conf_src conf_tgt. pcofix CIH. intros idx st_src st_tgt SIM. inv SIM.
-  pfold. punfold LOCAL. inv LOCAL.
-  - econs 1; eauto.
-  - (* return *)
-    destruct st2_src, st_tgt. ss.
-    destruct EC0, EC1. ss. subst.
-    inv STACK.
-    + (* final *)
-      admit.
-    + (* return *)
-      econs 3; ss.
-      { admit. (* tgt not stuck *) }
-      i. inv STEP0. rewrite returnUpdateLocals_spec in *. ss.
-      rewrite RET_TGT in *.
-      exploit LOCAL; eauto.
-      { instantiate (1 := Some _). ss. eauto. }
-      i. des.
-      esplits; eauto.
-      * econs 1. destruct conf_src. ss. econs; eauto.
-        { admit. (* free_allocas *) }
-        { rewrite returnUpdateLocals_spec, RET_SRC. eauto. }
-      * right. apply CIH. econs; eauto.
-        etransitivity; eauto.
-  - (* return_void *)
-    destruct st2_src, st_tgt. ss.
-    destruct EC0, EC1. ss. subst.
-    inv STACK.
-    + (* final *)
-      admit.
-    + (* return *)
-      econs 3; ss.
-      { admit. (* tgt not stuck *) }
-      i. inv STEP0.
-      destruct cmd_tgt; ss. destruct noret5; ss.
-      destruct cmd_src; ss. destruct noret5; ss.
-      exploit LOCAL; eauto.
-      { instantiate (1 := None). instantiate (1 := None). ss. }
-      i. des. inv RETURN_SRC.
-      esplits; eauto.
-      * econs 1. destruct conf_src. econs; eauto.
-        admit. (* free_allocas *)
-      * right. apply CIH. econs; eauto.
-        etransitivity; eauto.
-  - (* call *)
-    admit.
-  - econs 3; ss. i. exploit STEP; eauto. i. des.
-    inv SIM; [|done].
-    esplits; eauto. right.
-    apply CIH. econs; eauto.
-    etransitivity; eauto.
-Admitted.
